Validator/Regex/Memoize/Memoize.lean
@@ -28,11 +28,11 @@ instance (m: Type -> Type u) (σ: Type) [DecidableEq σ] [Hashable σ] [Monad m]
   enterM param := MemTable.enter (monadState := enterState) param
   leaveM param := MemTable.leave (monadState := leaveState) param
 
-def derive [Monad m] [DecidableEq σ] [Hashable σ] [MemoizeRoom m σ]
+def Regex.Memoize.derive [Monad m] [DecidableEq σ] [Hashable σ] [MemoizeRoom m σ]
   (Φ: σ → Bool) (r: Regex σ): m {dr: Regex σ // dr = Regex.Room.derive Φ r } := do
   let ⟨symbols, hsymbols⟩ <- MemoizeRoom.enterM r
   let ⟨res, hres⟩ <- MemoizeRoom.leaveM ⟨r, Vector.map Φ symbols⟩
-  let h: res = r.leave (Vector.map Φ r.enter) := by
+  let h: res = Regex.Room.derive Φ r := by
     unfold leave at hres
     simp only at hres
     rw [hsymbols] at hres
@@ -47,30 +47,30 @@ def StateMemoize.run {σ: Type} {β: Type} [DecidableEq σ] [Hashable σ]
   (state: memoizeState σ) (f: StateMemoize σ β): β :=
   ((StateM.run (StateT.run f state.1) state.2).1).1
 
-def StateMemoize.derive [DecidableEq σ] [Hashable σ] (Φ: σ → Bool) (r: Regex σ): StateMemoize σ (Regex σ) :=
+def StateMemoize.Regex.derive [DecidableEq σ] [Hashable σ] (Φ: σ → Bool) (r: Regex σ): StateMemoize σ (Regex σ) :=
   Regex.Memoize.derive Φ r
 
-def StateMemoize.derive.run {σ: Type} [DecidableEq σ] [Hashable σ]
+def StateMemoize.Regex.derive.run {σ: Type} [DecidableEq σ] [Hashable σ]
   (state: memoizeState σ) (Φ: σ → Bool) (r: Regex σ): Regex σ :=
   StateMemoize.run state (Regex.Memoize.derive Φ r)
 
-#guard StateMemoize.derive.run memoizeState.init
+#guard StateMemoize.Regex.derive.run memoizeState.init
   (· == 'a') (Regex.or (Regex.symbol 'a') (Regex.symbol 'b'))
   = Regex.or Regex.emptystr Regex.emptyset
 
 def validate [Monad m] [DecidableEq σ] [Hashable σ] [MemoizeRoom m σ]
   (Φ: σ → α → Bool) (r: Regex σ) (xs: List α): m Bool :=
-  null <$> (List.foldlM (fun dr x => derive (flip Φ x) dr) r xs)
+  null <$> (List.foldlM (fun dr x => Regex.Memoize.derive (flip Φ x) dr) r xs)
 
-def StateMemoize.validate [DecidableEq σ] [Hashable σ]
+def StateMemoize.Regex.validate [DecidableEq σ] [Hashable σ]
   (Φ: σ → α → Bool) (r: Regex σ) (xs: List α): StateMemoize σ Bool :=
   Regex.Memoize.validate Φ r xs
 
-def StateMemoize.validate.run {σ: Type} [DecidableEq σ] [Hashable σ]
+def StateMemoize.Regex.validate.run {σ: Type} [DecidableEq σ] [Hashable σ]
   (state: memoizeState σ) (Φ: σ → α → Bool) (r: Regex σ) (xs: List α): Bool :=
-  StateMemoize.run state (StateMemoize.validate Φ r xs)
+  StateMemoize.run state (StateMemoize.Regex.validate Φ r xs)
 
-#guard StateMemoize.validate.run memoizeState.init
+#guard StateMemoize.Regex.validate.run memoizeState.init
   (· == ·) (Regex.or (Regex.symbol 'a') (Regex.symbol 'b')) ['a']
   = true
 
@@ -78,34 +78,32 @@ def filter  [Monad m] [DecidableEq σ] [Hashable σ] [MemoizeRoom m σ]
   (Φ: σ → α → Bool) (r: Regex σ) (xss: List (List α)): m (List (List α)) :=
   List.filterM (validate Φ r) xss
 
-def StateMemoize.filter [DecidableEq σ] [Hashable σ]
+def StateMemoize.Regex.filter [DecidableEq σ] [Hashable σ]
   (Φ: σ → α → Bool) (r: Regex σ) (xss: List (List α)): StateMemoize σ (List (List α)) :=
   Regex.Memoize.filter Φ r xss
 
-def StateMemoize.filter.run [DecidableEq σ] [Hashable σ]
+def StateMemoize.Regex.filter.run [DecidableEq σ] [Hashable σ]
   (state: memoizeState σ)
   (Φ: σ → α → Bool) (r: Regex σ) (xss: List (List α)): List (List α) :=
-  StateMemoize.run state (StateMemoize.filter Φ r xss)
+  StateMemoize.run state (StateMemoize.Regex.filter Φ r xss)
 
-lemma StateMemoize.derive.run_unfold [DecidableEq σ] [Hashable σ]
+lemma StateMemoize.Regex.derive.run_unfold [DecidableEq σ] [Hashable σ]
   (state: memoizeState σ) (Φ: σ → Bool) (r: Regex σ):
-  (StateMemoize.derive.run state Φ r) = StateMemoize.run state (Memoize.derive Φ r) :=
+  (StateMemoize.Regex.derive.run state Φ r) = StateMemoize.run state (Regex.Memoize.derive Φ r) :=
   rfl
 
-theorem StateMemoize.derive.run_is_correct [DecidableEq σ] [Hashable σ]
+theorem StateMemoize.Regex.derive.run_is_correct [DecidableEq σ] [Hashable σ]
   (state: memoizeState σ)
   (Φ: σ → Bool) (r: Regex σ):
-  StateMemoize.derive.run state Φ r = Regex.Room.derive Φ r := by
-  rw [StateMemoize.derive.run_unfold]
-  generalize StateMemoize.run state (Memoize.derive Φ r) = x
+  StateMemoize.Regex.derive.run state Φ r = Regex.Room.derive Φ r := by
+  rw [StateMemoize.Regex.derive.run_unfold]
+  generalize StateMemoize.run state (Regex.Memoize.derive Φ r) = x
   obtain ⟨dr, hdr⟩ := x
   simp only
   rw [hdr]
 
-theorem StateMemoize.derive_commutes {σ: Type} {α: Type} [DecidableEq σ] [Hashable σ]
+theorem Regex.StateMemoize.derive_commutes {σ: Type} {α: Type} [DecidableEq σ] [Hashable σ]
   (state: memoizeState σ) (Φ: σ → α → Prop) [DecidableRel Φ] (r: Regex σ) (a: α):
-  denote Φ (StateMemoize.derive.run state (flip (decideRel Φ) a) r) = Lang.derive (denote Φ r) a := by
-  rw [StateMemoize.derive.run_is_correct]
-  rw [Regex.Room.derive_is_Regex_derive]
-  rw [<- Regex.derive_commutes]
-  congr
+  denote Φ (StateMemoize.Regex.derive.run state (flip (decideRel Φ) a) r) = Lang.derive (denote Φ r) a := by
+  rw [StateMemoize.Regex.derive.run_is_correct]
+  rw [<- Regex.Room.derive_commutes]
