Validator/Hedge.lean
@@ -1,6 +1,7 @@
 import Validator.Hedge.Denote
 import Validator.Hedge.Grammar
 import Validator.Hedge.Lang
+import Validator.Hedge.Memoize
 import Validator.Hedge.Original
 import Validator.Hedge.Room
 import Validator.Hedge.Types
