Validator/Hedge/Memoize/Memoize.lean
@@ -1,0 +1,247 @@
+import Mathlib.Tactic.SimpRw
+
+import Validator.Std.Decidable
+import Validator.Std.Hedge
+import Validator.Std.Vec
+
+import Validator.Regex.Lang
+import Validator.Regex.Room
+import Validator.Regex.Enter
+import Validator.Regex.Memoize.Memoize
+import Validator.Hedge.Denote
+import Validator.Hedge.Grammar
+import Validator.Hedge.Room
+import Validator.Hedge.Lang
+import Validator.Hedge.Denote
+
+import Validator.Regex.Memoize
+open Regex.Memoize
+
+
+namespace Hedge
+
+def Vec.mapM [Monad m] (g: α -> β) (f: (a: α) -> m {res // res = g a})  (xs: Vector α n)
+  : m (Vector β n) :=
+  Vector.mapM (fun a => (·.1) <$> (f a)) xs
+
+def List.mappyM [Monad m] {g: α -> β} (f: (a: α) -> m {res // res = g a}) (xs: List α)
+  : m {ys: (List β) // ys = List.map g xs } :=
+  match xs with
+  | [] => pure ⟨[], rfl⟩
+  | (x::xs') => do
+    let ⟨fx, hfx⟩ <- f x
+    let ⟨fxs, hfxs⟩ <- List.mappyM f xs'
+    pure (Subtype.mk (fx::fxs) (by
+      simp only [List.map]
+      rw [hfx]
+      rw [hfxs]
+    ))
+
+theorem eq (xs ys: Vector α n) (h: Vector.toList xs = Vector.toList ys): xs = ys := by
+  obtain ⟨⟨xs⟩, hxs⟩ := xs
+  obtain ⟨⟨ys⟩, hxs⟩ := ys
+  simp_all
+
+theorem take_toList (xs: Vector α l):
+  (Vector.take xs n).toList = List.take n xs.toList := by
+  -- exact?
+  exact Vector.toList_take
+
+theorem push_toList (xs: Vector α n) (x: α):
+  (Vector.push xs x).toList = xs.toList ++ [x] := by
+  -- exact?
+  exact Vector.toList_push
+
+theorem size_eq_one:
+  (xs: Vector α (0 + 1)) -> ∃ x, xs = #v[x] := by
+  exact fun xs => Vector.size_eq_one
+
+theorem asdfasdfas (xs: List α) (hxs: (Vector.size (Vector.mk (Array.mk xs) rfl)) = n + 1) (hget : k < n + 1) (hget': k < xs.length):
+  (Vector.mk (Array.mk xs) hxs).get ⟨k, hget⟩ = List.get xs ⟨k, hget'⟩ := by
+  exact rfl
+
+theorem take1_toList (xs: Vector α (n + 1)) (h: k <= n):
+  (List.take (k + 1) xs.toList) = (List.take k (xs.toList)) ++ [xs.get ⟨k, by omega⟩] := by
+  obtain ⟨⟨xs⟩, hxs⟩ := xs
+  simp
+  generalize_proofs hget
+  have hk : k < xs.length := by
+    simp at hxs
+    omega
+  rw [asdfasdfas (hget' := hk)]
+  simp_all only [List.size_toArray, List.get_eq_getElem, List.take_append_getElem]
+
+def Vec.mapM' [Monad m] (g: α -> β) (f: (a: α) -> m {res // res = g a}) (xs : Vector α n)
+  : m {ys: (Vector β n) // ys = Vector.map g xs } := do
+  go 0 (Nat.zero_le n) ⟨#v[], by simp⟩
+where
+  go (k : Nat) (h : k ≤ n) (acc : {ys: (Vector β k) // ys = Vector.cast (by omega) (Vector.map g (Vector.take xs k)) })
+    : m {ys: (Vector β n) // ys = Vector.map g xs } := do
+      if h' : k < n then
+        f xs[k] >>=
+          fun xsk =>
+            go (k+1) (by omega) (⟨acc.val.push xsk, by
+              obtain ⟨acc, hacc⟩ := acc
+              simp only
+              rw [hacc]
+              obtain ⟨xsk, hxsk⟩ := xsk
+              simp only
+              rw [hxsk]
+              apply eq
+              rw [Vector.cast_toList]
+              rw [Vector.map_toList]
+              rw [take_toList]
+              rw [push_toList]
+              rw [Vector.cast_toList]
+              rw [Vector.map_toList]
+              rw [take_toList]
+              rw [<- hxsk]
+              -- generalize (xs.toList) = xs'
+              cases n with
+              | zero =>
+                contradiction
+              | succ n' =>
+                rw [take1_toList (h := by omega)]
+                rw [List.map_append]
+                congr
+          ⟩)
+      else
+        return ⟨Vector.cast (by omega) acc.val, by
+          generalize_proofs h1 h2
+          obtain ⟨acc, hacc⟩ := acc
+          simp only
+          rw [hacc]
+          aesop
+        ⟩
+
+def Regex.StateMemoize.deriveM [DecidableEq σ] [Hashable σ]
+  (Φ': σ -> Bool) (Φ: (s: σ) → StateMemoize σ { b // b = Φ' s }) (r: Regex σ):
+  StateMemoize σ {dr: Regex σ // dr = Regex.Room.derive Φ' r } := do
+  let ⟨symbols, hsymbols⟩ <- MemoizeRoom.enterM r
+  let bools <- Vec.mapM' Φ' Φ symbols
+  let ⟨res, hres⟩ <- MemoizeRoom.leaveM ⟨r, bools⟩
+  let h: res = Regex.Room.derive Φ' r := by
+    unfold leave at hres
+    simp only at hres
+    subst_eqs
+    rename_i hleave
+    obtain ⟨bools, hbools⟩ := bools
+    obtain ⟨leave, hleave⟩ := hleave
+    simp only
+    rw [hbools]
+    rfl
+  pure (Subtype.mk res h)
+
+def pureNodePred (G: Grammar n φ) (Φ: φ → α → Bool) (node: Node α) (symbol: (φ × Ref n)) :=
+    let ⟨label, children⟩ := node
+    let childr := if Φ symbol.1 label then G.lookup symbol.2 else Regex.emptyset
+    Regex.null (List.foldl (Grammar.Room.derive G Φ) childr children)
+
+def List.foldlM'' [Monad m] (g: β -> α -> β) (xs: List α)
+  (f: (acc: β) -> (a: {a': α // a' ∈ xs}) -> m {res: β // res = g acc a } )
+  (init: β)
+  : m {res': β // res' = List.foldl g init xs } :=
+  match xs with
+  | [] => pure ⟨init, rfl⟩
+  | (x::xs') => do
+    let fx <- f init (Subtype.mk x (by simp))
+    let fxs <- List.foldlM'' g xs' (fun acc a => do
+      let ⟨b, hb⟩ := a
+      let a'': { a' // a' ∈ x :: xs' } := Subtype.mk b (by
+        aesop
+      )
+      let f': { res // res = g acc a''.val } <- f acc a''
+      let f'': { res // res = g acc b } := by
+        subst a''
+        simp only at f'
+        assumption
+      pure f''
+    ) fx.val
+    pure (Subtype.mk fxs.val (by
+      obtain ⟨fxs, hfxs⟩ := fxs
+      simp only
+      obtain ⟨fx, hfx⟩ := fx
+      simp only at hfxs
+      rw [hfxs]
+      rw [hfx]
+      simp only
+      simp only [List.foldl]
+    ))
+
+def Grammar.Room.derive'' (G: Grammar n φ) (Φ: φ → α → Bool)
+  (r: Regex (φ × Ref n)) (node: Node α): Regex (φ × Ref n) :=
+  let nodePred: (param: φ × Ref n) → Bool := (fun ((labelPred, ref): (φ × Ref n)) =>
+    let ⟨label, children⟩ := node
+    let childr := if Φ labelPred label then G.lookup ref else Regex.emptyset
+    Regex.null (List.foldl (Grammar.Room.derive'' G Φ) childr children)
+  )
+  Regex.Room.derive nodePred r
+
+def Grammar.StateMemoize.derive' [DecidableEq α] [Hashable α] [DecidableEq φ] [Hashable φ]
+  (G: Grammar n φ) (Φ: φ → α → Bool)
+  (r: Regex (φ × Ref n)) (children: Hedge α) (node: { node': Node α // node' ∈ children}): StateMemoize (φ × Ref n) { dr: (Regex (φ × Ref n)) // dr = Grammar.Room.derive G Φ r node } := do
+  let nodePred: (param: φ × Ref n) → StateMemoize (φ × Ref n) {b: Bool // b = pureNodePred G Φ node.val param } :=
+    (fun ((labelPred, ref): (φ × Ref n)) =>
+      match hnode: node with
+      | Subtype.mk (Hedge.Node.mk label children) hhnode =>
+      let childr := if Φ labelPred label then G.lookup ref else Regex.emptyset
+      List.foldlM'' (Grammar.Room.derive G Φ) children (Grammar.StateMemoize.derive' G Φ (children := children)) childr >>=
+        fun dr =>
+          let dn: Bool := Regex.null dr.val
+          pure (Subtype.mk dn (by
+            obtain ⟨dr, hdr⟩ := dr
+            subst dn
+            simp only
+            rw [hdr]
+            unfold pureNodePred
+            simp only
+            subst childr
+            rfl
+          ))
+  )
+  let dr <- Regex.StateMemoize.deriveM (pureNodePred G Φ node) nodePred r
+  pure (Subtype.mk dr.val (by
+    obtain ⟨dr, hdr⟩ := dr
+    simp only
+    rw [hdr]
+    unfold Grammar.Room.derive
+    rfl
+  ))
+  termination_by node.val
+  decreasing_by
+    · obtain ⟨node, hnode⟩ := node
+      simp only
+      apply Node.sizeOf_children hnode
+
+def Grammar.StateMemoize.derive [DecidableEq α] [Hashable α] [DecidableEq φ] [Hashable φ]
+  (G: Grammar n φ) (Φ: φ → α → Bool)
+  (r: Regex (φ × Ref n)) (node: Node α): StateMemoize (φ × Ref n) { dr: (Regex (φ × Ref n)) // dr = Grammar.Room.derive G Φ r node } :=
+  Grammar.StateMemoize.derive' G Φ r [node] (Subtype.mk node (by simp))
+
+def StateMemoize.Grammar.derive.run {φ: Type} [DecidableEq φ] [Hashable φ] [DecidableEq α] [Hashable α]
+  (state: memoizeState (φ × Ref n)) (G: Grammar n φ) (Φ: φ → α → Bool) (r: Regex (φ × Ref n)) (node: Node α): Regex (φ × Ref n) :=
+  StateMemoize.run state (Grammar.StateMemoize.derive G Φ r node)
+
+lemma StateMemoize.Grammar.derive.run_unfold {φ: Type} [DecidableEq φ] [Hashable φ] [DecidableEq α] [Hashable α]
+  (state: memoizeState (φ × Ref n)) (G: Grammar n φ) (Φ: φ → α → Bool) (r: Regex (φ × Ref n)) (node: Node α):
+  (StateMemoize.Grammar.derive.run state G Φ r node) = StateMemoize.run state (Grammar.StateMemoize.derive G Φ r node) :=
+  rfl
+
+theorem StateMemoize.Grammar.derive.run_is_correct [DecidableEq φ] [Hashable φ] [DecidableEq α] [Hashable α]
+  (state: memoizeState (φ × Ref n))
+  (Φ: φ → α → Bool) (G: Grammar n φ) (r: Regex (φ × Ref n)) (node: Node α):
+  StateMemoize.Grammar.derive.run state G Φ r node = Grammar.Room.derive G Φ r node := by
+  rw [StateMemoize.Grammar.derive.run_unfold]
+  generalize StateMemoize.run state (Grammar.StateMemoize.derive G Φ r node) = x
+  obtain ⟨dr, hdr⟩ := x
+  simp only
+  rw [hdr]
+
+theorem StateMemoize.Grammar.derive_commutes [DecidableEq φ] [Hashable φ] [DecidableEq α] [Hashable α]
+  (state: memoizeState (φ × Ref n))
+  (Φ: φ → α → Prop) [DecidableRel Φ]
+  (G: Grammar n φ) (r: Regex (φ × Ref n)) (node: Node α):
+  Grammar.Rule.denote G Φ (StateMemoize.Grammar.derive.run state G (decideRel Φ) r node)
+  = Lang.derive (Grammar.Rule.denote G Φ r) node := by
+  rw [StateMemoize.Grammar.derive.run_is_correct]
+  rw [<- Grammar.Room.derive_commutes]
